formal/tlaplus/slashing/MC_SlashFlow.tla
@@ -1,7 +1,7 @@
 --------------------------- MODULE MC_SlashFlow ---------------------------
 (****************************************************************************)
 (* Model-checking instance for SlashFlow.                                   *)
-(* Three validators, each bonded with 100 stake; max seq number 3.          *)
+(* Three validators, each bonded with 100 stake; max seq number 2.          *)
 (****************************************************************************)
 
 EXTENDS SlashFlow, TLC
@@ -10,6 +10,6 @@ CONSTANTS v1, v2, v3
 
 MC_Validators    == {v1, v2, v3}
 MC_InitialBonds  == (v1 :> 100 @@ v2 :> 100 @@ v3 :> 100)
-MC_MaxSeqNum     == 3
+MC_MaxSeqNum     == 2
 
 ============================================================================
